fixed rand test

rand_test.ec
@@ -1,62 +1,168 @@
 prover quorum=2 ["Alt-Ergo" "Z3"].
-timeout 2.  (* limit SMT solvers to two seconds *)
-require import AllCore Distr.
+timeout 1.  (* limit SMT solvers to two seconds *)
+require import AllCore FSet List Distr.
+require import Bool IntDiv.
+require import Number StdOrder.
+(*---*) import RealOrder. 
 
-op randint : int distr.
-axiom randint_ll : is_lossless randint.
+const order : { int | 2 <= order } as ge2_order.
 
-(* bitwidth of int *)
-op L : int.
-axiom ge0_L : 0 <= L.
+require import ZModP. 
+clone import ZModField as Zmod with op p <- order.
 
-axiom randint1E (x : int) :
-  mu1 randint x = 1%r / (2 ^ L)%r.
+import Zmod.Sub.
+import Zmod.ZModule.
 
-axiom uniform_randint : is_uniform randint.
+require (*---*) DynMatrix.
 
-lemma randint_full : is_full randint.
-proof.
-move => x.
-rewrite /support randint1E.
-by rewrite RField.div1r StdOrder.RealOrder.invr_gt0 lt_fromint StdOrder.IntOrder.expr_gt0.
-qed.
+
+clone DynMatrix as Mat_A with
+type ZR.t <- Zmod.zmod,
+pred ZR.unit   <- Zmod.unit,
+op ZR.zeror  <- Zmod.zero,
+op ZR.oner   <- Zmod.one,
+op ZR.( + )  <- Zmod.( + ),
+op ZR.([-])  <- Zmod.([-]),
+op ZR.( * )  <- Zmod.( * ),
+op ZR.invr   <- Zmod.inv,
+op ZR.exp    <- Zmod.exp
+
+proof ZR.addrA by exact Zmod.ZModpField.addrA,
+ZR.addrC by exact Zmod.ZModpField.addrC,
+ZR.add0r by exact Zmod.ZModpField.add0r,
+ZR.addNr by exact Zmod.ZModpField.addNr,
+ZR.oner_neq0 by exact Zmod.ZModpField.oner_neq0,
+ZR.mulrA by exact Zmod.ZModpField.mulrA,
+ZR.mulrC by exact Zmod.ZModpField.mulrC,
+ZR.mul1r by exact Zmod.ZModpField.mul1r,
+ZR.mulrDl by exact Zmod.ZModpField.mulrDl,
+ZR.mulVr by exact Zmod.ZModpRing.mulVr,
+ZR.mulrV by exact Zmod.ZModpRing.mulrV,
+ZR.unitP by exact Zmod.ZModpRing.unitP,
+ZR.unitout by exact Zmod.ZModpRing.unitout,
+ZR.expr0 by exact Zmod.ZModpRing.expr0,
+ZR.exprS by exact Zmod.ZModpRing.exprS,
+ZR.exprN by exact Zmod.ZModpRing.exprN.
+
+import Zmod.DZmodP.
+
+op randint : zmod distr = dunifin.
 
 module M = {
-  proc f() : int = {
-    var a, b : int;
+  proc f() : zmod = {
+    var a, b : zmod;
     a <$ randint;
     b <$ randint;
     return a + b;
   }
 
-  proc g() : int = {
-    var r : int;
+  proc g() : zmod = {
+    var r : zmod;
     r <$ randint;
     return r;
   }
 }.
 
-op rnd_f : int -> int.
-op rnd_g : int -> int.
+lemma randint_full: is_full randint by exact dunifin_fu.
+
+lemma randint1E (s : zmod) : mu1 randint s = (1%r / order%r)%Real
+  by rewrite dunifin1E cardE.
+
+lemma randint_ll: is_lossless randint by exact dunifin_ll.
+
+lemma randint_funi: is_funiform randint.
+proof.
+by move=> ??; rewrite !randint1E.
+qed.
+
+op rnd_f : zmod -> zmod.
+op rnd_g : zmod -> zmod.
 
 axiom f_inv : forall x, rnd_f (rnd_f x) = x.
 axiom fg_inv : forall x, rnd_f (rnd_g x) = x.
 axiom gf_inv : forall x, rnd_g (rnd_f x) = x.
+
+lemma addS (a b c : zmod) :
+    a - b = c <=> a = b + c.
+proof.
+smt(addrA addrC addNr add0r).
+qed.
+
+lemma subrr (x : zmod) :
+    x - x = zero.
+proof.
+smt(addNr add0r).
+qed.
+
+lemma subK (a b : zmod) :
+  a - (a - b) = b.
+proof.
+by rewrite addS -addrA addNr addrC add0r.
+qed.
 
 lemma indist :
     equiv[M.f ~ M.g : true ==> ={res}].
 proof.
 proc.
 (* consume the first random assignment *)
+seq 1 0 : true.
 rnd{1}.
-rnd rnd_f rnd_g.
+auto.
+rnd (fun u => a{1} + u) (fun u => u - a{1}).
 auto.
 progress.
-by rewrite fg_inv.
-smt(randint1E).
-rewrite randint_full.
-by rewrite gf_inv.
-rewrite randint_ll.
-(* ???? *)
+by rewrite -addS.
+smt(addrC addrA subrr).
+qed.
+
+(* without seq, it doesn't work *)
+lemma indist_stuck :
+    equiv[M.f ~ M.g : true ==> ={res}].
+proof.
+proc.
+rnd{1}.
+rnd (fun u => a{1} + u) (fun u => u - a{1}).
+auto; progress.
+by rewrite -addS.
+smt(addrC addrA subrr).
+(* stuck: aL + b0 = a{1} + aL *)
 admit.
+qed.
+
+op randint2 : int distr.
+
+module M2 = {
+  proc f() : int = {
+    var a, b : int;
+    a <$ randint2;
+    b <$ randint2;
+    return a + b;
+  }
+
+  proc g() : int = {
+    var r : int;
+    r <$ randint2;
+    return r;
+  }
+}.
+
+lemma indist2 :
+    equiv[M2.f ~ M2.g : true ==> ={res}].
+proof.
+proc.
+(* consume the first random assignment *)
+seq 1 0 : true.
+rnd{1}.
+auto.
+(* not true: is_lossless randint2 *)
+admit.
+rnd (fun u => a{1} + u) (fun u => u - a{1}).
+auto.
+progress.
+smt().
+(* not true mu1 r = mu1 r - a *)
+admit.
+(* maybe true: randint full *)
+admit.
+smt().
 qed.
